

Computer Vision

Module 5-6

②(a) Derive the motion tracking equation from fundamental principles.

⇒ Brightness constancy

$$I(x + \delta x, y + \delta y, t + \Delta t) \approx I(x, y, t) \quad \text{--- (1)}$$

⇒ Taylor Series Expansion

$$I(x + \delta x, y + \delta y, t + \Delta t) \approx I(x, y, t) + \frac{\partial I}{\partial x} \delta x + \frac{\partial I}{\partial y} \delta y$$

⇒ Optical Flow constraint

$$+ \frac{\partial I}{\partial t} \Delta t \quad \text{--- (2)}$$

Substituting (2) in (1)

$$I(x, y, t) + \frac{\partial I}{\partial x} \delta x + \frac{\partial I}{\partial y} \delta y + \frac{\partial I}{\partial t} \Delta t \approx I(x, y, t)$$

$$\frac{\partial I}{\partial x} \delta x + \frac{\partial I}{\partial y} \delta y + \frac{\partial I}{\partial t} \Delta t \approx 0$$

⇒ Motion Tracking Equation

$$I_x = \frac{\partial I}{\partial x} \quad (\text{Gradient along } x)$$

$$I_y = \frac{\partial I}{\partial y} \quad (\text{Gradient along } y)$$

$$I_t = \frac{\partial I}{\partial t} \quad (\text{Gradient along } t)$$

$$u = \frac{\delta x}{\Delta t}, \quad v = \frac{\delta y}{\Delta t}$$

$$\frac{\partial I}{\partial x} \cdot \frac{\delta x}{\Delta t} + \frac{\partial I}{\partial y} \frac{\delta y}{\Delta t} + \frac{\partial I}{\partial t} \frac{\Delta t}{\Delta t} \approx 0$$

$$I_x u + I_y v + I_t \approx 0$$

$$I_x u + I_y v \approx -I_t$$

$$I_{x1}u + I_{y1}v \approx -I_{t1}$$

$$I_{x2}u + I_{y2}v \approx -I_{t2}$$

$$I_{xn}u + I_{yn}v \approx -I_{tn}$$

$$A\bar{m} = b$$

$$\begin{bmatrix} I_{x1} & I_{y1} \\ I_{x2} & I_{y2} \\ \vdots & \vdots \\ I_{xn} & I_{yn} \end{bmatrix}_{n \times 2} \begin{bmatrix} u \\ v \end{bmatrix}_{2 \times 1} = \begin{bmatrix} -I_{t1} \\ -I_{t2} \\ \vdots \\ -I_{tn} \end{bmatrix}_{n \times 1}$$

$$\bar{m} = A^{-1}b$$

$$\bar{m}A^T = A^{-1}A^Tb$$

$$\bar{m} = (A^TA)^{-1}A^Tb$$

$$A^TA = \begin{bmatrix} I_{x1} & I_{x2} & \dots & I_{xn} \\ I_{y1} & I_{y2} & \dots & I_{yn} \end{bmatrix}_{2 \times n} \begin{bmatrix} I_{x1} & I_{y1} \\ I_{x2} & I_{y2} \\ \vdots & \vdots \\ I_{xn} & I_{yn} \end{bmatrix}_{n \times 2}$$

$$= \begin{bmatrix} \sum_{i=1}^n I_{xi}^2 & \sum_{i=1}^n I_{xi} I_{yi} \\ \sum_{i=1}^n I_{yi} I_{xi} & \sum_{i=1}^n I_{yi}^2 \end{bmatrix}_{2 \times 2}$$

$$A^T b = \begin{bmatrix} I_{x1} & I_{x2} & \dots & I_{xn} \\ I_{y1} & I_{y2} & \dots & I_{yn} \end{bmatrix}_{2 \times n} \begin{bmatrix} -I_{t1} \\ -I_{t2} \\ \vdots \\ -I_{tn} \end{bmatrix}_{n \times 1}$$

$$= \begin{bmatrix} \sum_{i=1}^n -I_{xi} I_{ti} \\ \sum_{i=1}^n -I_{yi} I_{ti} \end{bmatrix}_{1 \times 1}$$

$$m = \left(\begin{bmatrix} \sum_{i=1}^n I_{xi}^2 & \sum_{i=1}^n I_{xi} I_{yi} \\ \sum_{i=1}^n I_{yi} I_{xi} & \sum_{i=1}^n I_{yi}^2 \end{bmatrix} \right)^{-1} \begin{bmatrix} \sum_{i=1}^n -I_{xi} I_{ti} \\ \sum_{i=1}^n -I_{yi} I_{ti} \end{bmatrix}$$

$$\begin{bmatrix} u \\ v \end{bmatrix} = \frac{1}{\det(A^T A)} \begin{bmatrix} \sum_{i=1}^n I_{yi}^2 & -\sum_{i=1}^n I_{xi} I_{yi} \\ -\sum_{i=1}^n I_{yi} I_{xi} & \sum_{i=1}^n I_{xi}^2 \end{bmatrix} \begin{bmatrix} -\sum_{i=1}^n I_{xi} I_{ti} \\ -\sum_{i=1}^n I_{yi} I_{ti} \end{bmatrix}$$